new/proof/go_etcd_io/etcd/client/v3/leasing.v
@@ -10,7 +10,8 @@ Require Import New.proof.go_etcd_io.etcd.client.v3.
 
 Class leasingG Σ :=
   {
-    concurrency_inG :: concurrencyG Σ
+    concurrency_inG :: concurrencyG Σ;
+    context_inG :: contextG Σ
   }.
 
 Section proof.
@@ -150,28 +151,49 @@ Proof.
   }
   rewrite decide_True //. wp_auto.
   iNamed "Hown".
-  wp_auto. wp_if_destruct.
-  2:{ (* not nil *)
-    wp_auto.
-    wp_apply "HDone".
-    ltac2:(wp_bind_apply ()).
-    iApply wp_Session__Done.
-    {
-      iSplitR.
-      { solve_pkg_init. (* FIXME: solve_pkg_init is pretty slow here. *) }
-      iFrame "#".
-    }
-    iNext. iIntros "* #HsessDone".
-    wp_auto.
-    wp_apply wp_chan_select_blocking.
-    rewrite big_andL_cons.
-    iSplit.
-    2:{
-      rewrite big_andL_cons. rewrite big_andL_nil.
-      iSplit; last done.
+  wp_auto.
+  wp_bind (if: _ then _ else _)%E.
+  iApply (wp_wand _ _ _ (λ v,
+                           (⌜ v = execute_val #tt ⌝ ∨
+                                    ⌜ v = return_val #tt ⌝) ∗
+                           "session" ∷ _ ↦s[_::_]{#1/2} session0 ∗ _)%I with "[-]").
+  {
+    wp_if_destruct.
+    { simpl. iFrame "session". iSplitR.
+      { by iLeft. }
+      iNamedAccu. }
+    { (* not nil *)
+      wp_auto.
+      wp_apply "HDone".
+      ltac2:(wp_bind_apply ()).
+      iApply wp_Session__Done.
+      {
+        iSplitR.
+        { solve_pkg_init. (* FIXME: solve_pkg_init is pretty slow here. *) }
+        iFrame "#".
+      }
+      iNext. iIntros "* #HsessDone".
+      wp_auto.
+      wp_apply wp_chan_select_blocking.
+      rewrite big_andL_cons.
+      iSplit.
+      2:{
+        rewrite big_andL_cons. rewrite big_andL_nil.
+        iSplit; last done.
+        repeat iExists _.
+        iApply (closeable_chan_receive with "HDone_ch").
+        iIntros "_". simpl. wp_auto. iFrame. by iRight.
+      }
       repeat iExists _.
+      iApply (closeable_chan_receive with "HsessDone").
+      iIntros "_". wp_auto. iFrame. by iLeft.
     }
-Qed.
+  }
+  iIntros "* ([%|%] & H)"; subst; iNamed "H".
+  2:{ wp_auto. wp_for_post. by iApply "HΦ". }
+  wp_auto.
+  (* Acquire lock, etc. *)
+Admitted.
 
 Lemma wp_NewKV cl γetcd (pfx : go_string) opts_sl :
   {{{
@@ -184,10 +206,16 @@ Lemma wp_NewKV cl γetcd (pfx : go_string) opts_sl :
 Proof.
   wp_start. iNamed "Hpre".
   wp_auto.
-  wp_apply (wp_Client__Ctx with "[$]") as "% _".
+  wp_apply (wp_Client__Ctx with "[$]") as "* #Hctx".
   iDestruct (is_Client_to_pub with "[$]") as "#Hclient_pub".
   iNamed "Hclient_pub".
-  wp_apply (wp_WithCancel with "[$]").
+  wp_apply (wp_WithCancel with "[]").
+  { iFrame "#".
+    iExactEq "Hctx".
+    repeat f_equal.
+    Print gFunctors.
+    (* FIXME: two different [contextG] instances are available in context. *)
+  }
   iIntros "* #(Hctx' & Hcancel_spec & Hctx_done)".
   wp_auto.
   unshelve wp_apply wp_map_make as "%revokes Hrevokes"; try tc_solve; try tc_solve.
